Adding other instances

CoqOfRust/pinocchio/links/instruction.v
@@ -268,8 +268,7 @@ Module Impl_From_ref_slice_u8_for_Seed.
   Proof.
     eexists.
     { eapply IsTraitMethod.Defined.
-      { with_strategy transparent [Φ] cbn.
-        apply pinocchio.instruction.instruction.Impl_core_convert_From_ref__slice_u8_for_pinocchio_instruction_Seed.Implements. }
+      { apply pinocchio.instruction.instruction.Impl_core_convert_From_ref__slice_u8_for_pinocchio_instruction_Seed.Implements. }
       { reflexivity. } }
     { constructor.
       admit. }
@@ -279,3 +278,24 @@ Module Impl_From_ref_slice_u8_for_Seed.
     : From.Run Seed.t (Ref.t Pointer.Kind.Ref (list (Integer.t IntegerKind.U8))) :=
     { From.from := run_from }.
 End Impl_From_ref_slice_u8_for_Seed.
+
+Print pinocchio.instruction.instruction.Impl_core_convert_From_ref__array_SIZE_u8_for_pinocchio_instruction_Seed.
+
+Module Impl_From_ref_array_u8_SIZE_for_Seed.
+  Definition run_from
+    : forall (SIZE : Usize.t),
+      From.Run_from Seed.t (Ref.t Pointer.Kind.Ref (array.t (Integer.t IntegerKind.U8) SIZE)).
+  Proof.
+    intros SIZE.
+    eexists.
+    { eapply IsTraitMethod.Defined.
+      { apply pinocchio.instruction.instruction.Impl_core_convert_From_ref__array_SIZE_u8_for_pinocchio_instruction_Seed.Implements. }
+      { reflexivity. } }
+    { constructor.
+      admit. }
+  Admitted.
+
+  Instance run (SIZE : Usize.t)
+    : From.Run Seed.t (Ref.t Pointer.Kind.Ref (array.t (Integer.t IntegerKind.U8) SIZE)) :=
+    { From.from := run_from SIZE }.
+End Impl_From_ref_array_u8_SIZE_for_Seed.
